Update Sequent.thy

Sequent.thy
@@ -10,7 +10,7 @@ section \<open>Terms and formulae\<close>
 text \<open>
 \label{sec:terms} The datatypes of terms and formulae are defined as follows:
 \<close>
-datatype ('f) tm  = Var nat | Fresh nat |  Fun 'f \<open>nat list\<close> 
+datatype ('f) tm  = Var nat  |  Fun 'f \<open>'f tm list\<close> 
 
 datatype sign = pos | neg
 
@@ -29,11 +29,11 @@ subsection \<open>Fresh term\<close>
 
 fun fresh_var :: "nat => 'f tm => bool" where
   "fresh_var x (Var y) = (x \<noteq> y)" |
-  "fresh_var x (Fun f xs) = (list_all (\<lambda>a. a = x) xs)" 
+  "fresh_var x (Fun f xs) = (list_all (\<lambda>a. fresh_var x a) xs)" 
 
 primrec deX :: "'f tm => nat list" where 
   "deX (Var n) = [n] "|
-  "deX (Fun f xs) = xs"
+  "deX (Fun f xs) = (concat (map deX xs))"
 
 definition
   freshVar :: "string tm list => string tm" where
@@ -45,19 +45,20 @@ lemma "freshVar [Var (0::nat), Var 1, Var 3] = Var 2"
 
 subsection \<open>Semantics of term and form\<close>
 
-primrec semantics_tm :: "(nat \<Rightarrow> string) \<Rightarrow> ('f \<Rightarrow> string list \<Rightarrow> string) \<Rightarrow> 'f tm \<Rightarrow> string" (\<open>\<lparr>_, _\<rparr>\<close>) where
-  \<open>\<lparr>E, F\<rparr> (Var n) = E n\<close> |
-  \<open>\<lparr>E, F\<rparr> (Fresh n) = E n\<close> |
-  \<open>\<lparr>E, F\<rparr> (Fun f ts) = F f (map E ts)\<close>
+primrec semantics_term and semantics_list where
+  \<open>semantics_term e f (Var n) = e n\<close> |
+  \<open>semantics_term e f (Fun i l) = f i (semantics_list e f l)\<close> |
+  \<open>semantics_list e f [] = []\<close> |
+  \<open>semantics_list e f (t # l) = semantics_term e f t # semantics_list e f l\<close>
 
 fun concat_str :: "string \<Rightarrow> string list \<Rightarrow> string" where
   "concat_str s ls = (if s = ''concat'' then List.concat ls else [])"
 
 primrec semantics_fm (\<open>\<lbrakk>_, _\<rbrakk>\<close>) where
-  \<open>\<lbrakk>E, F\<rbrakk> (EqAtom s x y) = (if s = pos then \<lparr>E, F\<rparr> x = \<lparr>E, F\<rparr> y else \<lparr>E, F\<rparr> x \<noteq> \<lparr>E, F\<rparr> y)\<close> 
+  \<open>\<lbrakk>E, F\<rbrakk> (EqAtom s x y) = (if s = pos then semantics_term E F x = semantics_term E F y else semantics_term E F x \<noteq> semantics_term E F y)\<close> 
 | \<open>\<lbrakk>E, F\<rbrakk> (EqFresh s x y) = True\<close> 
-| \<open>\<lbrakk>E, F\<rbrakk> (ConcEq z x y) = (\<lparr>E, F\<rparr> z = \<lparr>E, F\<rparr> x @ \<lparr>E, F\<rparr> y)\<close> 
-| \<open>\<lbrakk>E, F\<rbrakk> (Member s x r) = (if s = pos then \<lparr>E, F\<rparr> x \<in> lang r else \<lparr>E, F\<rparr> x \<notin> lang r)\<close> 
+| \<open>\<lbrakk>E, F\<rbrakk> (ConcEq z x y) = (semantics_term E F z = semantics_term E F x @ semantics_term E F y)\<close> 
+| \<open>\<lbrakk>E, F\<rbrakk> (Member s x r) = (if s = pos then semantics_term E F x \<in> lang r else semantics_term E F x \<notin> lang r)\<close> 
 | \<open>\<lbrakk>E, F\<rbrakk> (Dis x y) = (\<lbrakk>E, F\<rbrakk> x \<or> \<lbrakk>E, F\<rbrakk> y)\<close> 
 | \<open>\<lbrakk>E, F\<rbrakk> (Con x y) = (\<lbrakk>E, F\<rbrakk> x \<and> \<lbrakk>E, F\<rbrakk> y)\<close> 
 | \<open>\<lbrakk>E, F\<rbrakk> (Neg x) = (\<not> \<lbrakk>E, F\<rbrakk> x)\<close> 
@@ -86,7 +87,7 @@ fun exists_solution :: "string form list \<Rightarrow> bool" where
                        else list_all is_Member ls \<and> distinct_variable ls \<and> single_word ls)"  
 
 fun empty_intersection_set :: "char BA rexp list \<Rightarrow> bool" where
-  "empty_intersection_set fs = (\<Inter>(lang ` set fs) = {} \<and> length fs > 1 )"
+  "empty_intersection_set fs = (\<Inter>(lang ` set fs) = {})"
 
 fun subset_intersect_set :: "char BA rexp \<Rightarrow> char BA rexp list \<Rightarrow> bool" where 
   "subset_intersect_set r fs = (\<Inter>(lang ` set fs) \<subseteq> lang r)"
@@ -100,7 +101,7 @@ fun member_var_rexp :: "nat list \<Rightarrow> char BA rexp list \<Rightarrow> s
   "member_var_rexp (x#xs) (y#ys) = (if (length xs = length ys) then (Member pos (Var x) y) # (member_var_rexp xs ys) else [])"
 
 fun con_fwd_prop ::"char BA rexp \<Rightarrow> char BA rexp \<Rightarrow> char BA rexp \<Rightarrow> bool" where
-  "con_fwd_prop r e1 r2 = (lang (r) = lang (Times e1 r2))"
+  "con_fwd_prop r r1 r2 = (lang r = lang (Times r1 r2))"
 
 fun con_fwd_prop_elim ::"char BA rexp \<Rightarrow> char BA rexp \<Rightarrow> char BA rexp \<Rightarrow> bool" where
   "con_fwd_prop_elim r e1 e2 = (lang r = lang (Times e1 e2) \<and> is_singleton (lang r))"
@@ -115,32 +116,45 @@ inductive One_SC :: \<open>string form list \<Rightarrow> bool\<close> (\<open>\
 | AlphaNegAnd:   \<open>\<stileturn> Neg A # \<Gamma> \<Longrightarrow>  \<stileturn> Neg B # \<Gamma> \<Longrightarrow> \<stileturn> Neg (Con A B) # \<Gamma>\<close>
 | AlphaNegNeg:   \<open>\<stileturn> A# \<Gamma> \<Longrightarrow> \<stileturn> Neg (Neg A) # \<Gamma>\<close>
 | NotMember:     \<open>regexp_compl e ec \<Longrightarrow> \<stileturn> (Member pos x ec) # \<Gamma> \<Longrightarrow> \<stileturn> (Member neg x e) # \<Gamma>\<close>
-| NotEq:         \<open>y = freshVar ([x,(Fun f xs)])  \<Longrightarrow> \<stileturn> [EqFresh neg x y,  EqFresh pos y (Fun f xs), \<Gamma>] \<Longrightarrow> \<stileturn> [EqAtom neg x (Fun f xs), \<Gamma>]\<close>
+| NotEq:         \<open>\<stileturn> [EqFresh neg x y,  EqFresh pos y (Fun f xs), \<Gamma>] \<Longrightarrow> \<stileturn> [EqAtom neg x (Fun f xs), \<Gamma>]\<close>
 | Cut:           \<open>regexp_compl e ec \<Longrightarrow> \<stileturn> Member pos x e # \<Gamma> \<Longrightarrow>  \<stileturn> Member pos x ec # \<Gamma> \<Longrightarrow>  \<stileturn> \<Gamma>\<close>
 | EqProp:        \<open>\<stileturn> Member pos x e # EqAtom pos x y # Member pos y e # \<Gamma> \<Longrightarrow> \<stileturn> Member pos x e # EqAtom pos x y # \<Gamma>\<close>
 | NeqSubsume:    \<open>regexp_empty e1 e2 \<Longrightarrow> \<stileturn> Member pos x e1 # Member pos y e2 # \<Gamma> \<Longrightarrow> \<stileturn> Member pos x e1 # EqAtom neg x y # Member pos y e2 # \<Gamma>\<close>
 | EqPropElim:    \<open>is_singleton (lang e) \<Longrightarrow> \<stileturn> Member pos x e # Member pos y e # \<Gamma>\<Longrightarrow> \<stileturn> Member pos x e # (EqAtom pos x y) # \<Gamma>\<close>
 | NeqPropElim:   \<open>is_singleton (lang e) \<Longrightarrow> regexp_compl e ec \<Longrightarrow> \<stileturn> (Member pos x e) # (Member pos y ec) # \<Gamma> \<Longrightarrow>  
                  \<stileturn> (Member pos x e) # (EqAtom neg x y) # \<Gamma>\<close>
-| Close:         \<open>empty_intersection_set rs \<Longrightarrow> \<stileturn> map (\<lambda>r. Member pos x r) rs\<close> 
+| Close:         \<open>length rs > 1 \<Longrightarrow> empty_intersection_set rs \<Longrightarrow> \<stileturn> (map (\<lambda>r. Member pos x r) rs) @ \<Gamma>\<close> 
 | Subsume:       \<open>subset_intersect_set e fs \<Longrightarrow> \<stileturn> (map (\<lambda>r. Member pos x r) fs) @ \<Gamma> \<Longrightarrow> \<stileturn> Member pos x e # (map (\<lambda>r. Member pos x r) fs) @ \<Gamma>\<close> 
 | Intersect:     \<open>eq_len_intersect e fs \<Longrightarrow> \<stileturn> Member pos x e # \<Gamma>  \<Longrightarrow>  \<stileturn> (map (\<lambda>r. Member pos x r) (fs)) @ \<Gamma>\<close> 
-| Fwd_PropConc:  \<open>con_fwd_prop e e1 e2 \<Longrightarrow> \<stileturn> [(Member pos x e), (EqAtom pos x (Fun ''concat'' [x1,x2])), (Member pos (Var x1) e1), (Member pos (Var x2) e2)] @ \<Gamma>
-                 \<Longrightarrow> \<stileturn> [(EqAtom pos x (Fun ''concat'' [x1,x2])), (Member pos (Var x1) e1), (Member pos (Var x2) e2)] @ \<Gamma>\<close>  
-| Fwd_ElimConc:  \<open>con_fwd_prop_elim e e1 e2 \<Longrightarrow> \<stileturn> [Member pos x e, (Member pos (Var x1) e1), (Member pos (Var x2) e2)]  @ \<Gamma> \<Longrightarrow>  
-                 \<stileturn> [(EqAtom pos x (Fun ''concat'' [x1, x2])), (Member pos (Var x1) e1), (Member pos (Var x2) e2)] @ \<Gamma>\<close>
-(*| Bwd_PropConc:  \<open>con_bwd_prop e = es \<Longrightarrow> \<stileturn> ((\<lambda>r. [Member x e, EqAtom x (Fun ''concat'' [x1,x2]), Member (Var x1) (fst r), Member (Var x2) (snd r)] @ \<Gamma>) ` es) \<Longrightarrow> 
+| Fwd_PropConc:  \<open>con_fwd_prop e e1 e2 \<Longrightarrow> \<stileturn> [(Member pos x e), (EqAtom pos x (Fun ''concat'' [x1,x2])), (Member pos (x1) e1), (Member pos (x2) e2)] @ \<Gamma>
+                 \<Longrightarrow> \<stileturn> [(EqAtom pos x (Fun ''concat'' [x1,x2])), (Member pos (x1) e1), (Member pos (x2) e2)] @ \<Gamma>\<close>  
+| Fwd_ElimConc:  \<open>con_fwd_prop_elim e e1 e2 \<Longrightarrow> \<stileturn> [Member pos x e, (Member pos (x1) e1), (Member pos (x2) e2)]  @ \<Gamma> \<Longrightarrow>  
+                 \<stileturn> [(EqAtom pos x (Fun ''concat'' [x1, x2])), (Member pos (x1) e1), (Member pos (x2) e2)] @ \<Gamma>\<close>
+(*| Bwd_PropConc:  \<open>con_bwd_prop e = es \<Longrightarrow> \<stileturn> ((\<lambda>r. [Member x e, EqAtom x (Fun ''concat'' [x1,x2]), Member (x1) (fst r), Member (x2) (snd r)] @ \<Gamma>) ` es) \<Longrightarrow> 
                  \<stileturn> {[Member x e, EqAtom x (Fun ''concat'' [x1,x2])] @ \<Gamma>}\<close>*)
 | Order:         \<open>\<stileturn> G \<Longrightarrow> set G = set G' \<Longrightarrow> \<stileturn> G'\<close>
-| Basic:        \<open> \<stileturn> [A,Neg A, G]\<close>
-| BasicFF: \<open>\<stileturn> FF # G\<close>
+| Basic:         \<open>\<stileturn> [A,Neg A, G]\<close>
+| BasicFF:       \<open>\<stileturn> FF # G\<close>
 
 declare One_SC.intros [intro]
 
 subsection \<open>Soundness\<close>
 
+lemma aux_close : "Suc 0 < |rs| \<Longrightarrow>  \<Inter> (Symbolic_Regular_Algebra_Model.lang ` set rs) = {} \<Longrightarrow> \<exists>p\<in>Member pos x ` set rs . \<not> \<lbrakk>E, \<lambda>a b. if a = ''concat'' then concat b else []\<rbrakk> p"
+  apply auto
+  done
+
 lemma SC_soundness: \<open>\<stileturn> G \<Longrightarrow> (\<exists>p \<in> set G. \<not> \<lbrakk>E, concat_str\<rbrakk> p)\<close>
 proof (induct G rule: One_SC.induct)
+  case (Close rs x \<Gamma>)
+  then show ?case apply auto
+  proof -
+    assume a1:"Suc 0 < |rs|" and a2:"\<Inter> (Symbolic_Regular_Algebra_Model.lang ` set rs) = {}"
+    then have "\<exists>p\<in>Member pos x ` set rs. \<not> \<lbrakk>E, \<lambda>a b. if a = ''concat'' then concat b else []\<rbrakk> p" by auto
+    then show "\<exists>p\<in>Member pos x ` set rs \<union> set \<Gamma>. \<not> \<lbrakk>E, \<lambda>a b. if a = ''concat'' then concat b else []\<rbrakk> p" 
+      by blast
+  qed
+next
   case (Intersect e fs x \<Gamma>)
   then show ?case  apply auto 
     by (smt (verit) INT_I image_subset_iff semantics_fm.simps(4) sup.cobounded1)
@@ -167,18 +181,18 @@ definition consistency :: "string form set set \<Rightarrow> bool" where
               (\<forall> A B. Dis A B \<in> S \<longrightarrow> S \<union> {A} \<in> C \<or> S \<union> {B} \<in> C) \<and> 
               (\<forall> A B. Neg (Con A B) \<in> S \<longrightarrow> S \<union> {Neg A} \<in> C \<or> S \<union> {Neg B} \<in> C) \<and> 
               (\<forall> A. Neg (Neg A) \<in> S \<longrightarrow> S \<union> {A} \<in> C) \<and> 
-              (\<forall> x e ec. regexp_compl e ec \<longrightarrow> Member neg x e \<in> S \<longrightarrow> S \<union> {Member pos x ec} \<in> C ) \<and> 
-              (\<forall> x y f xs. EqAtom neg  x (Fun f xs) \<in> S \<longrightarrow> S \<union> {EqAtom neg  x y, EqAtom pos y (Fun f xs)} \<in> C) \<and> 
-              (\<forall> x e ec. regexp_compl e ec \<longrightarrow> S \<union> {Member pos x e} \<in> C \<or> S \<union> {Member pos x ec} \<in> C) \<and> 
+              (\<forall> x e ec. regexp_compl e ec \<longrightarrow> Member neg x e \<in> S \<longrightarrow> S \<union> {Member pos x ec} \<in> C) \<and> 
+              (\<forall> x y f xs. EqAtom neg  x (Fun f xs) \<in> S \<longrightarrow> S \<union> {EqFresh neg  x y, EqFresh pos y (Fun f xs)} \<in> C) \<and> 
+              (\<forall> x e ec. regexp_compl e ec \<longrightarrow> S \<union> {Member pos x e} \<in> C \<longrightarrow> S \<union> {Member pos x ec} \<in> C) \<and> 
               (\<forall> x y e. Member pos x e \<in> S \<and> EqAtom pos x y \<in> S \<longrightarrow> S \<union> {Member pos x e, EqAtom pos x y, Member pos y e} \<in> C) \<and> 
               (\<forall> e1 e2 x y. regexp_empty e1 e2 \<longrightarrow> Member pos x e1 \<in> S \<and> EqAtom neg  x y \<in> S \<and> Member pos y e2 \<in> S \<longrightarrow> S \<union> {Member pos x e1, Member pos y e2} \<in> C) \<and>
               (\<forall> x y e. is_singleton (lang e) \<longrightarrow> Member pos x e \<in> S \<and> EqAtom pos x y \<in> S \<longrightarrow> S \<union> {Member pos x e, Member pos y e} \<in> C) \<and> 
               (\<forall> x y e ec. is_singleton (lang e) \<longrightarrow> regexp_compl e ec \<longrightarrow> Member pos x e \<in> S \<and> EqAtom neg  x y \<in> S \<longrightarrow> S \<union> {Member pos x e, Member pos y ec} \<in> C) \<and> 
-              (\<forall> x rs. empty_intersection_set rs \<longrightarrow> S \<union> ((\<lambda>r. Member pos x r) ` (set rs)) \<in> C \<longrightarrow> S \<union> {FF} \<in> C) \<and> 
+              (\<forall> x rs. length rs > 1 \<longrightarrow> empty_intersection_set rs \<longrightarrow> S \<union> ((\<lambda>r. Member pos x r) ` (set rs)) \<notin> C) \<and> 
               (\<forall> x e fs. subset_intersect_set e fs \<longrightarrow> Member pos x e \<in> S \<and> S \<union> ((\<lambda>r. Member pos x r)) ` (set fs) \<in> C \<longrightarrow> S \<union> ((\<lambda>r. Member pos x r)) ` (set fs) \<in> C) \<and> 
               (\<forall> x e fs. eq_len_intersect e fs \<longrightarrow>  S \<union> ((\<lambda>r. Member pos x r)) ` (set fs) \<in> C \<longrightarrow> S \<union> {Member pos x e} \<in> C) \<and> 
-              (\<forall> x x1 x2 e e1 e2 f. con_fwd_prop e e1 e2 \<longrightarrow> EqAtom pos x (Fun f [x1, x2]) \<in> S \<and> Member pos (Var x1) e1 \<in> S \<and> Member pos (Var x2) e2 \<in> S \<longrightarrow> S \<union> {Member pos x e, EqAtom pos x (Fun f [x1,x2]), Member pos (Var x1) e1, Member pos (Var x2) e2} \<in> C) \<and> 
-              (\<forall> x x1 x2 e e1 e2 f. con_fwd_prop_elim e e1 e2 \<longrightarrow> EqAtom pos x (Fun f [x1, x2]) \<in> S \<and> Member pos (Var x1) e1 \<in> S \<and> Member pos (Var x2) e2 \<in> S \<longrightarrow> S \<union> {Member pos x e, Member pos (Var x1) e1, Member pos (Var x2) e2} \<in> C) \<and> 
+              (\<forall> x x1 x2 e e1 e2. con_fwd_prop e e1 e2 \<longrightarrow> EqAtom pos x (Fun ''concat'' [x1, x2]) \<in> S \<and> Member pos (x1) e1 \<in> S \<and> Member pos (x2) e2 \<in> S \<longrightarrow> S \<union> {Member pos x e, EqAtom pos x (Fun ''concat'' [x1,x2]), Member pos (x1) e1, Member pos (x2) e2} \<in> C) \<and> 
+              (\<forall> x x1 x2 e e1 e2. con_fwd_prop_elim e e1 e2 \<longrightarrow> EqAtom pos x (Fun ''concat'' [x1, x2]) \<in> S \<and> Member pos (x1) e1 \<in> S \<and> Member pos (x2) e2 \<in> S \<longrightarrow> S \<union> {EqAtom pos x (Fun ''concat'' [x1,x2]), Member pos x e, Member pos (x1) e1, Member pos (x2) e2} \<in> C) \<and> 
               (\<forall> S'. S' = S \<longrightarrow> S' \<in> C))"
 
 subsection \<open>Completeness\<close>
@@ -243,10 +257,77 @@ proof (intro conjI allI impI notI)
   {
     fix x y f xs 
     assume \<open>EqAtom neg x (Fun f xs) \<in> S\<close>
-    then show \<open>S \<union> {EqAtom neg x y, EqAtom pos y (Fun f xs)} \<in> {set G |G. \<not> (\<stileturn> G)}\<close>
-      using * \<open>\<not> (\<stileturn> G)\<close> Order NotEq apply auto
+    then show \<open>S \<union> {EqFresh neg x y, EqFresh pos y (Fun f xs)} \<in> {set G |G. \<not> (\<stileturn> G)}\<close>
+      using * \<open>\<not> (\<stileturn> G)\<close> Order NotEq apply auto  sorry
+  }
+  {
+    fix x y e
+    assume \<open>Member pos x e \<in> S \<and> EqAtom pos x y \<in> S\<close>
+    then show \<open>S \<union> {Member pos x e, EqAtom pos x y, Member pos y e} \<in> {set G |G. \<not> (\<stileturn> G)}\<close>
+      using * \<open>\<not> (\<stileturn> G)\<close> Order EqProp apply auto 
       by (metis insert_absorb list.simps(15))
   }
+  {
+    fix e1 e2 x y
+    assume \<open>regexp_empty e1 e2\<close> and \<open>Member pos x e1 \<in> S \<and> EqAtom neg x y \<in> S \<and> Member pos y e2 \<in> S\<close>
+    then show \<open>S \<union> {Member pos x e1, Member pos y e2} \<in> {set G |G. \<not> (\<stileturn> G)}\<close>
+      using * \<open>\<not> (\<stileturn> G)\<close> Order NeqSubsume apply auto done
+  }
+  {
+    fix x y e
+    assume \<open>is_singleton (Symbolic_Regular_Algebra_Model.lang e)\<close> and \<open>Member pos x e \<in> S \<and> EqAtom pos x y \<in> S\<close>
+    then show \<open>S \<union> {Member pos x e, Member pos y e} \<in> {set G |G. \<not> (\<stileturn> G)}\<close>
+      using * \<open>\<not> (\<stileturn> G)\<close> Order EqPropElim apply auto 
+      by (metis insert_absorb list.simps(15))
+  }
+  {
+    fix x y e ec
+    assume \<open>is_singleton (Symbolic_Regular_Algebra_Model.lang e)\<close> and
+       \<open>regexp_compl e ec\<close> and
+       \<open>Member pos x e \<in> S \<and> EqAtom neg x y \<in> S\<close>
+    then show \<open>S \<union> {Member pos x e, Member pos y ec} \<in> {set G |G. \<not> (\<stileturn> G)}\<close>
+      using * \<open>\<not> (\<stileturn> G)\<close> Order NeqPropElim apply auto 
+      by (metis insert_absorb list.simps(15))
+  }
+  {
+    fix x rs
+    assume \<open> 1 < |rs|\<close> and \<open>empty_intersection_set rs\<close> and  \<open>S \<union> Member pos x ` set rs \<in> {set G |G. \<not> (\<stileturn> G)}\<close>
+    then show False
+      using * \<open>\<not> (\<stileturn> G)\<close> Order Close apply auto 
+      by (metis list.set_map set_append sup_commute)
+  }
+  {
+    fix x e fs
+    assume \<open>subset_intersect_set e fs\<close> and \<open>Member pos x e \<in> S \<and> S \<union> Member pos x ` set fs \<in> {set G |G. \<not> (\<stileturn> G)}\<close>
+    then show \<open>S \<union> Member pos x ` set fs \<in> {set G |G. \<not> (\<stileturn> G)}\<close>
+      using * \<open>\<not> (\<stileturn> G)\<close> Order Subsume apply auto done
+  }
+  {
+    fix x e fs
+    assume \<open>eq_len_intersect e fs\<close> and \<open>S \<union> Member pos x ` set fs \<in> {set G |G. \<not> (\<stileturn> G)}\<close>
+    then show \<open>S \<union> {Member pos x e} \<in> {set G |G. \<not> (\<stileturn> G)}\<close>
+      using * \<open>\<not> (\<stileturn> G)\<close> Order Intersect apply auto 
+      by (metis List.insert_def List.set_insert list.set_map set_append sup_commute)
+  }
+  {
+    fix x x1 x2 e e1 e2
+    assume \<open>con_fwd_prop e e1 e2\<close> and \<open>EqAtom pos x (Fun ''concat'' [x1, x2]) \<in> S \<and> Member pos x1 e1 \<in> S \<and> Member pos x2 e2 \<in> S\<close>
+    then show \<open>S \<union> {Member pos x e, EqAtom pos x (Fun ''concat'' [x1, x2]), Member pos x1 e1, Member pos x2 e2} \<in> {set G |G. \<not> (\<stileturn> G)}\<close>
+      using * \<open>\<not> (\<stileturn> G)\<close> Order Fwd_PropConc apply auto sorry
+  }
+  {
+    fix S'
+    assume \<open>S \<in> {set G |G. \<not> (\<stileturn> G)}\<close> and \<open>S' = S\<close>
+    then show \<open>S' \<in> {set G |G. \<not> (\<stileturn> G)}\<close>
+      using * \<open>\<not> (\<stileturn> G)\<close> Order apply auto  done
+  }
+  {
+    fix x x1 x2 e e1 e2 
+    assume \<open>con_fwd_prop_elim e e1 e2\<close> and \<open>EqAtom pos x (Fun ''concat'' [x1, x2]) \<in> S \<and> Member pos x1 e1 \<in> S \<and> Member pos x2 e2 \<in> S\<close>
+    then show \<open>S \<union> {EqAtom pos x (Fun ''concat'' [x1,x2]), Member pos x e, Member pos x1 e1, Member pos x2 e2} \<in> {set G |G. \<not> (\<stileturn> G)}\<close>
+      using * \<open>\<not> (\<stileturn> G)\<close> Order Fwd_ElimConc apply auto sorry
+  }
+
 
 
 
